try to prove preservation

Core/Lemmas.v
@@ -1,7 +1,575 @@
 From Stdlib Require Import Lists.List.
+From Stdlib Require Import Strings.String.
 From DOMLCore Require Import Syntax Context Substitution Typing Operational Automation.
 
 Import ListNotations.
+
+Inductive appears_free_in : var -> tm -> Prop :=
+| AF_Var : forall x,
+    appears_free_in x (tVar x)
+| AF_Let1 : forall x y e1 e2,
+    appears_free_in x e1 ->
+    appears_free_in x (tLet y e1 e2)
+| AF_Let2 : forall x y e1 e2,
+    x <> y ->
+    appears_free_in x e2 ->
+    appears_free_in x (tLet y e1 e2)
+| AF_Pi1 : forall x y T U,
+    appears_free_in x T ->
+    appears_free_in x (tPi y T U)
+| AF_Pi2 : forall x y T U,
+    x <> y ->
+    appears_free_in x U ->
+    appears_free_in x (tPi y T U)
+| AF_Lam1 : forall x y T e,
+    appears_free_in x T ->
+    appears_free_in x (tLam y T e)
+| AF_Lam2 : forall x y T e,
+    x <> y ->
+    appears_free_in x e ->
+    appears_free_in x (tLam y T e)
+| AF_App1 : forall x e1 e2,
+    appears_free_in x e1 ->
+    appears_free_in x (tApp e1 e2)
+| AF_App2 : forall x e1 e2,
+    appears_free_in x e2 ->
+    appears_free_in x (tApp e1 e2)
+| AF_Sigma1 : forall x y T U,
+    appears_free_in x T ->
+    appears_free_in x (tSigma y T U)
+| AF_Sigma2 : forall x y T U,
+    x <> y ->
+    appears_free_in x U ->
+    appears_free_in x (tSigma y T U)
+| AF_Pair1 : forall x e1 e2,
+    appears_free_in x e1 ->
+    appears_free_in x (tPair e1 e2)
+| AF_Pair2 : forall x e1 e2,
+    appears_free_in x e2 ->
+    appears_free_in x (tPair e1 e2)
+| AF_Fst : forall x e,
+    appears_free_in x e ->
+    appears_free_in x (tFst e)
+| AF_Snd : forall x e,
+    appears_free_in x e ->
+    appears_free_in x (tSnd e)
+| AF_Sum1 : forall x T U,
+    appears_free_in x T ->
+    appears_free_in x (tSum T U)
+| AF_Sum2 : forall x T U,
+    appears_free_in x U ->
+    appears_free_in x (tSum T U)
+| AF_Inl1 : forall x U e,
+    appears_free_in x U ->
+    appears_free_in x (tInl U e)
+| AF_Inl2 : forall x U e,
+    appears_free_in x e ->
+    appears_free_in x (tInl U e)
+| AF_Inr1 : forall x T e,
+    appears_free_in x T ->
+    appears_free_in x (tInr T e)
+| AF_Inr2 : forall x T e,
+    appears_free_in x e ->
+    appears_free_in x (tInr T e)
+| AF_CaseScrut : forall x e y el z er,
+    appears_free_in x e ->
+    appears_free_in x (tCase e y el z er)
+| AF_CaseLeft : forall x e y el z er,
+    x <> y ->
+    appears_free_in x el ->
+    appears_free_in x (tCase e y el z er)
+| AF_CaseRight : forall x e y el z er,
+    x <> z ->
+    appears_free_in x er ->
+    appears_free_in x (tCase e y el z er)
+| AF_EqTy : forall x T e1 e2,
+    appears_free_in x T ->
+    appears_free_in x (tEq T e1 e2)
+| AF_EqLeft : forall x T e1 e2,
+    appears_free_in x e1 ->
+    appears_free_in x (tEq T e1 e2)
+| AF_EqRight : forall x T e1 e2,
+    appears_free_in x e2 ->
+    appears_free_in x (tEq T e1 e2)
+| AF_Refl : forall x e,
+    appears_free_in x e ->
+    appears_free_in x (tRefl e)
+| AF_EqElimP : forall x P e e' p q,
+    appears_free_in x P ->
+    appears_free_in x (tEqElim P e e' p q)
+| AF_EqElimLeft : forall x P e e' p q,
+    appears_free_in x e ->
+    appears_free_in x (tEqElim P e e' p q)
+| AF_EqElimRight : forall x P e e' p q,
+    appears_free_in x e' ->
+    appears_free_in x (tEqElim P e e' p q)
+| AF_EqElimProof : forall x P e e' p q,
+    appears_free_in x p ->
+    appears_free_in x (tEqElim P e e' p q)
+| AF_EqElimBody : forall x P e e' p q,
+    appears_free_in x q ->
+    appears_free_in x (tEqElim P e e' p q)
+| AF_Plus1 : forall x e1 e2,
+    appears_free_in x e1 ->
+    appears_free_in x (tPlus e1 e2)
+| AF_Plus2 : forall x e1 e2,
+    appears_free_in x e2 ->
+    appears_free_in x (tPlus e1 e2)
+| AF_Minus1 : forall x e1 e2,
+    appears_free_in x e1 ->
+    appears_free_in x (tMinus e1 e2)
+| AF_Minus2 : forall x e1 e2,
+    appears_free_in x e2 ->
+    appears_free_in x (tMinus e1 e2).
+
+Definition closed (e : tm) : Prop :=
+  forall x, ~ appears_free_in x e.
+
+Inductive wf_context (Delta : dom_context) (Omega : const_context) : context -> Prop :=
+| WF_Empty : wf_context Delta Omega []
+| WF_Extend : forall Gamma x T s,
+    wf_context Delta Omega Gamma ->
+    closed T ->
+    has_type Delta Omega Gamma T (tSort s) ->
+    wf_context Delta Omega (extend Gamma x T).
+
+Definition closed_context (Gamma : context) : Prop :=
+  forall x T, lookup x Gamma = Some T -> closed T.
+
+Lemma closed_context_empty :
+  closed_context [].
+Proof.
+  intros x T Hlookup. discriminate.
+Qed.
+
+Definition context_equiv (Gamma Gamma' : context) : Prop :=
+  forall x, lookup x Gamma = lookup x Gamma'.
+
+Lemma context_equiv_refl :
+  forall Gamma,
+    context_equiv Gamma Gamma.
+Proof.
+  intros Gamma x. reflexivity.
+Qed.
+
+Lemma context_equiv_extend :
+  forall Gamma Gamma' x T,
+    context_equiv Gamma Gamma' ->
+    context_equiv (extend Gamma x T) (extend Gamma' x T).
+Proof.
+  intros Gamma Gamma' x T Heq y.
+  unfold extend. simpl.
+  destruct (String.eqb y x); auto.
+Qed.
+
+Lemma typing_context_equiv :
+  forall Delta Omega Gamma Gamma' e T,
+    context_equiv Gamma Gamma' ->
+    has_type Delta Omega Gamma e T ->
+    has_type Delta Omega Gamma' e T.
+Proof.
+  intros Delta Omega Gamma Gamma' e T Heq HT.
+  generalize dependent Gamma'.
+  induction HT; intros Gamma' Heq; try solve [constructor; eauto].
+  - apply T_Var. rewrite <- Heq. assumption.
+  - eapply T_Let.
+    + apply IHHT1. assumption.
+    + apply IHHT2. assumption.
+    + apply IHHT3. apply context_equiv_extend. assumption.
+  - eapply T_Pi.
+    + apply IHHT1. assumption.
+    + apply IHHT2. apply context_equiv_extend. assumption.
+  - eapply T_Lam.
+    + apply IHHT1. assumption.
+    + apply IHHT2. apply context_equiv_extend. assumption.
+  - eapply T_App.
+    + apply IHHT1. assumption.
+    + apply IHHT2. assumption.
+  - eapply T_Sigma.
+    + apply IHHT1. assumption.
+    + apply IHHT2. apply context_equiv_extend. assumption.
+  - eapply T_Pair.
+    + apply IHHT1. assumption.
+    + apply IHHT2. assumption.
+    + apply IHHT3. assumption.
+  - eapply T_Fst. apply IHHT. assumption.
+  - eapply T_Snd. apply IHHT. assumption.
+  - eapply T_Inl.
+    + apply IHHT1. assumption.
+    + apply IHHT2. assumption.
+    + apply IHHT3. assumption.
+  - eapply T_Inr.
+    + apply IHHT1. assumption.
+    + apply IHHT2. assumption.
+    + apply IHHT3. assumption.
+  - eapply T_Case.
+    + apply IHHT1. assumption.
+    + apply IHHT2. apply context_equiv_extend. assumption.
+    + apply IHHT3. apply context_equiv_extend. assumption.
+  - eapply T_Eq.
+    + apply IHHT1. assumption.
+    + apply IHHT2. assumption.
+    + apply IHHT3. assumption.
+  - eapply T_Refl.
+    + apply IHHT1. assumption.
+    + apply IHHT2. assumption.
+  - eapply T_EqElim.
+    + apply IHHT1. assumption.
+    + apply IHHT2. assumption.
+    + apply IHHT3. assumption.
+  - eapply T_DomainType.
+    + eauto.
+    + apply IHHT1. assumption.
+    + apply IHHT2. assumption.
+  - eapply T_IntroDom.
+    + eauto.
+    + apply IHHT1. assumption.
+    + apply IHHT2. assumption.
+    + apply IHHT3. assumption.
+  - eapply T_Conv.
+    + apply IHHT. assumption.
+    + assumption.
+Qed.
+
+Lemma wf_context_tail :
+  forall Delta Omega Gamma x T,
+    wf_context Delta Omega (extend Gamma x T) ->
+    wf_context Delta Omega Gamma.
+Proof.
+  intros Delta Omega Gamma x T Hwf.
+  inversion Hwf; subst. assumption.
+Qed.
+
+Lemma wf_context_head_closed :
+  forall Delta Omega Gamma x T,
+    wf_context Delta Omega (extend Gamma x T) ->
+    closed T.
+Proof.
+  intros Delta Omega Gamma x T Hwf.
+  inversion Hwf; subst. assumption.
+Qed.
+
+Lemma wf_context_closed_context :
+  forall Delta Omega Gamma,
+    wf_context Delta Omega Gamma ->
+    closed_context Gamma.
+Proof.
+  intros Delta Omega Gamma Hwf.
+  induction Hwf; unfold closed_context in *; intros y U Hlookup.
+  - discriminate.
+  - unfold extend in Hlookup. simpl in Hlookup.
+    destruct (String.eqb_spec y x) as [Heq | Hneq].
+    + inversion Hlookup; subst. assumption.
+    + eapply IHHwf. exact Hlookup.
+Qed.
+
+Lemma closed_context_extend :
+  forall Gamma x T,
+    closed_context Gamma ->
+    closed T ->
+    closed_context (extend Gamma x T).
+Proof.
+  intros Gamma x T Hctx HT y U Hlookup.
+  unfold extend in Hlookup. simpl in Hlookup.
+  destruct (String.eqb_spec y x) as [Heq | Hneq].
+  - inversion Hlookup; subst. assumption.
+  - eapply Hctx. exact Hlookup.
+Qed.
+
+Lemma lookup_shadow :
+  forall Gamma x U T,
+    lookup x (extend (extend Gamma x U) x T) = Some T.
+Proof.
+  intros. apply lookup_extend_eq.
+Qed.
+
+Lemma lookup_drop_shadow :
+  forall Gamma x U T y,
+    lookup y (extend (extend Gamma x U) x T) =
+    lookup y (extend Gamma x T).
+Proof.
+  intros Gamma x U T y.
+  unfold extend. simpl.
+  destruct (String.eqb y x); reflexivity.
+Qed.
+
+Lemma typing_drop_shadow :
+  forall Delta Omega Gamma x U T e V,
+    has_type Delta Omega (extend (extend Gamma x U) x T) e V ->
+    has_type Delta Omega (extend Gamma x T) e V.
+Proof.
+  intros Delta Omega Gamma x U T e V HT.
+  eapply typing_context_equiv; [| exact HT].
+  intros y. apply lookup_drop_shadow.
+Qed.
+
+Lemma typing_shadow_weaken :
+  forall Delta Omega Gamma x U T e V,
+    has_type Delta Omega (extend Gamma x T) e V ->
+    has_type Delta Omega (extend (extend Gamma x U) x T) e V.
+Proof.
+  intros Delta Omega Gamma x U T e V HT.
+  eapply typing_context_equiv; [| exact HT].
+  intros y. symmetry. apply lookup_drop_shadow.
+Qed.
+
+Lemma closed_app_inv :
+  forall e1 e2,
+    closed (tApp e1 e2) -> closed e1 /\ closed e2.
+Proof.
+  intros e1 e2 H. split; unfold closed in *; intros x Hfree; apply (H x).
+  - apply AF_App1. exact Hfree.
+  - apply AF_App2. exact Hfree.
+Qed.
+
+Lemma closed_let_bound_inv :
+  forall y e1 e2,
+    closed (tLet y e1 e2) -> closed e1.
+Proof.
+  intros y e1 e2 H. unfold closed in *. intros x Hfree. apply (H x).
+  apply AF_Let1. exact Hfree.
+Qed.
+
+Lemma closed_pi_domain_inv :
+  forall y T U,
+    closed (tPi y T U) -> closed T.
+Proof.
+  intros y T U H. unfold closed in *. intros x Hfree. apply (H x).
+  apply AF_Pi1. exact Hfree.
+Qed.
+
+Lemma closed_lam_type_inv :
+  forall y T e,
+    closed (tLam y T e) -> closed T.
+Proof.
+  intros y T e H. unfold closed in *. intros x Hfree. apply (H x).
+  apply AF_Lam1. exact Hfree.
+Qed.
+
+Lemma closed_sigma_domain_inv :
+  forall y T U,
+    closed (tSigma y T U) -> closed T.
+Proof.
+  intros y T U H. unfold closed in *. intros x Hfree. apply (H x).
+  apply AF_Sigma1. exact Hfree.
+Qed.
+
+Lemma closed_pair_inv :
+  forall e1 e2,
+    closed (tPair e1 e2) -> closed e1 /\ closed e2.
+Proof.
+  intros e1 e2 H. split; unfold closed in *; intros x Hfree; apply (H x).
+  - apply AF_Pair1. exact Hfree.
+  - apply AF_Pair2. exact Hfree.
+Qed.
+
+Lemma closed_fst_inv :
+  forall e,
+    closed (tFst e) -> closed e.
+Proof.
+  intros e H. unfold closed in *. intros x Hfree. apply (H x).
+  apply AF_Fst. exact Hfree.
+Qed.
+
+Lemma closed_snd_inv :
+  forall e,
+    closed (tSnd e) -> closed e.
+Proof.
+  intros e H. unfold closed in *. intros x Hfree. apply (H x).
+  apply AF_Snd. exact Hfree.
+Qed.
+
+Lemma closed_sum_inl_inv :
+  forall U e,
+    closed (tInl U e) -> closed U /\ closed e.
+Proof.
+  intros U e H. split; unfold closed in *; intros x Hfree; apply (H x).
+  - apply AF_Inl1. exact Hfree.
+  - apply AF_Inl2. exact Hfree.
+Qed.
+
+Lemma closed_sum_inr_inv :
+  forall T e,
+    closed (tInr T e) -> closed T /\ closed e.
+Proof.
+  intros T e H. split; unfold closed in *; intros x Hfree; apply (H x).
+  - apply AF_Inr1. exact Hfree.
+  - apply AF_Inr2. exact Hfree.
+Qed.
+
+Lemma closed_case_inv :
+  forall e x el y er,
+    closed (tCase e x el y er) -> closed e.
+Proof.
+  intros e x el y er H. unfold closed in *. intros z Hfree. apply (H z).
+  apply AF_CaseScrut. exact Hfree.
+Qed.
+
+Lemma closed_refl_inv :
+  forall e,
+    closed (tRefl e) -> closed e.
+Proof.
+  intros e H. unfold closed in *. intros x Hfree. apply (H x).
+  apply AF_Refl. exact Hfree.
+Qed.
+
+Lemma closed_eqelim_inv :
+  forall P e e' p q,
+    closed (tEqElim P e e' p q) ->
+    closed P /\ closed e /\ closed e' /\ closed p /\ closed q.
+Proof.
+  intros P e e' p q H. repeat split; unfold closed in *; intros x Hfree;
+    apply (H x).
+  - apply AF_EqElimP. exact Hfree.
+  - apply AF_EqElimLeft. exact Hfree.
+  - apply AF_EqElimRight. exact Hfree.
+  - apply AF_EqElimProof. exact Hfree.
+  - apply AF_EqElimBody. exact Hfree.
+Qed.
+
+Lemma closed_plus_inv :
+  forall e1 e2,
+    closed (tPlus e1 e2) -> closed e1 /\ closed e2.
+Proof.
+  intros e1 e2 H. split; unfold closed in *; intros x Hfree; apply (H x).
+  - apply AF_Plus1. exact Hfree.
+  - apply AF_Plus2. exact Hfree.
+Qed.
+
+Lemma closed_minus_inv :
+  forall e1 e2,
+    closed (tMinus e1 e2) -> closed e1 /\ closed e2.
+Proof.
+  intros e1 e2 H. split; unfold closed in *; intros x Hfree; apply (H x).
+  - apply AF_Minus1. exact Hfree.
+  - apply AF_Minus2. exact Hfree.
+Qed.
+
+Lemma subst_not_free :
+  forall e x s,
+    ~ appears_free_in x e ->
+    subst x s e = e.
+Proof.
+  induction e; intros x s Hnot; simpl; try reflexivity.
+  - destruct (String.eqb_spec x v) as [Heq | Hneq].
+    + subst. exfalso. apply Hnot. constructor.
+    + reflexivity.
+  - f_equal.
+    + apply IHe1. intros Hfree. apply Hnot. apply AF_Let1. exact Hfree.
+    + destruct (String.eqb_spec x v) as [Heq | Hneq].
+      * reflexivity.
+      * apply IHe2. intros Hfree. apply Hnot.
+        apply AF_Let2; assumption.
+  - f_equal.
+    + apply IHe1. intros Hfree. apply Hnot. apply AF_Pi1. exact Hfree.
+    + destruct (String.eqb_spec x v) as [Heq | Hneq].
+      * reflexivity.
+      * apply IHe2. intros Hfree. apply Hnot.
+        apply AF_Pi2; assumption.
+  - f_equal.
+    + apply IHe1. intros Hfree. apply Hnot. apply AF_Lam1. exact Hfree.
+    + destruct (String.eqb_spec x v) as [Heq | Hneq].
+      * reflexivity.
+      * apply IHe2. intros Hfree. apply Hnot.
+        apply AF_Lam2; assumption.
+  - f_equal.
+    + apply IHe1. intros Hfree. apply Hnot. apply AF_App1. exact Hfree.
+    + apply IHe2. intros Hfree. apply Hnot. apply AF_App2. exact Hfree.
+  - f_equal.
+    + apply IHe1. intros Hfree. apply Hnot. apply AF_Sigma1. exact Hfree.
+    + destruct (String.eqb_spec x v) as [Heq | Hneq].
+      * reflexivity.
+      * apply IHe2. intros Hfree. apply Hnot.
+        apply AF_Sigma2; assumption.
+  - f_equal.
+    + apply IHe1. intros Hfree. apply Hnot. apply AF_Pair1. exact Hfree.
+    + apply IHe2. intros Hfree. apply Hnot. apply AF_Pair2. exact Hfree.
+  - f_equal. apply IHe. intros Hfree. apply Hnot. apply AF_Fst. exact Hfree.
+  - f_equal. apply IHe. intros Hfree. apply Hnot. apply AF_Snd. exact Hfree.
+  - f_equal.
+    + apply IHe1. intros Hfree. apply Hnot. apply AF_Sum1. exact Hfree.
+    + apply IHe2. intros Hfree. apply Hnot. apply AF_Sum2. exact Hfree.
+  - f_equal.
+    + apply IHe1. intros Hfree. apply Hnot. apply AF_Inl1. exact Hfree.
+    + apply IHe2. intros Hfree. apply Hnot. apply AF_Inl2. exact Hfree.
+  - f_equal.
+    + apply IHe1. intros Hfree. apply Hnot. apply AF_Inr1. exact Hfree.
+    + apply IHe2. intros Hfree. apply Hnot. apply AF_Inr2. exact Hfree.
+  - f_equal.
+    + apply IHe1. intros Hfree. apply Hnot. apply AF_CaseScrut. exact Hfree.
+    + destruct (String.eqb_spec x v) as [Heq | Hneq].
+      * reflexivity.
+      * apply IHe2. intros Hfree. apply Hnot.
+        apply AF_CaseLeft; assumption.
+    + destruct (String.eqb_spec x v0) as [Heq | Hneq].
+      * reflexivity.
+      * apply IHe3. intros Hfree. apply Hnot.
+        apply AF_CaseRight; assumption.
+  - f_equal.
+    + apply IHe1. intros Hfree. apply Hnot. apply AF_EqTy. exact Hfree.
+    + apply IHe2. intros Hfree. apply Hnot. apply AF_EqLeft. exact Hfree.
+    + apply IHe3. intros Hfree. apply Hnot. apply AF_EqRight. exact Hfree.
+  - f_equal. apply IHe. intros Hfree. apply Hnot. apply AF_Refl. exact Hfree.
+  - f_equal.
+    + apply IHe1. intros Hfree. apply Hnot. apply AF_EqElimP. exact Hfree.
+    + apply IHe2. intros Hfree. apply Hnot. apply AF_EqElimLeft. exact Hfree.
+    + apply IHe3. intros Hfree. apply Hnot. apply AF_EqElimRight. exact Hfree.
+    + apply IHe4. intros Hfree. apply Hnot. apply AF_EqElimProof. exact Hfree.
+    + apply IHe5. intros Hfree. apply Hnot. apply AF_EqElimBody. exact Hfree.
+  - f_equal.
+    + apply IHe1. intros Hfree. apply Hnot. apply AF_Plus1. exact Hfree.
+    + apply IHe2. intros Hfree. apply Hnot. apply AF_Plus2. exact Hfree.
+  - f_equal.
+    + apply IHe1. intros Hfree. apply Hnot. apply AF_Minus1. exact Hfree.
+    + apply IHe2. intros Hfree. apply Hnot. apply AF_Minus2. exact Hfree.
+Qed.
+
+Lemma subst_closed :
+  forall e x s,
+    closed e ->
+    subst x s e = e.
+Proof.
+  intros e x s Hclosed. apply subst_not_free. apply Hclosed.
+Qed.
+
+Lemma subst_replacement_defeq :
+  forall e x s s',
+    defeq s s' ->
+    defeq (subst x s e) (subst x s' e).
+Proof.
+  induction e; intros x s s' Hdef; simpl; try apply DE_Refl.
+  - destruct (String.eqb x v); [assumption | apply DE_Refl].
+  - apply DE_Let.
+    + apply IHe1. assumption.
+    + destruct (String.eqb x v); [apply DE_Refl | apply IHe2; assumption].
+  - apply DE_Pi.
+    + apply IHe1. assumption.
+    + destruct (String.eqb x v); [apply DE_Refl | apply IHe2; assumption].
+  - apply DE_Lam.
+    + apply IHe1. assumption.
+    + destruct (String.eqb x v); [apply DE_Refl | apply IHe2; assumption].
+  - apply DE_App; [apply IHe1 | apply IHe2]; assumption.
+  - apply DE_Sigma.
+    + apply IHe1. assumption.
+    + destruct (String.eqb x v); [apply DE_Refl | apply IHe2; assumption].
+  - apply DE_Pair; [apply IHe1 | apply IHe2]; assumption.
+  - apply DE_Fst. apply IHe. assumption.
+  - apply DE_Snd. apply IHe. assumption.
+  - apply DE_Sum; [apply IHe1 | apply IHe2]; assumption.
+  - apply DE_Inl; [apply IHe1 | apply IHe2]; assumption.
+  - apply DE_Inr; [apply IHe1 | apply IHe2]; assumption.
+  - apply DE_Case.
+    + apply IHe1. assumption.
+    + destruct (String.eqb x v); [apply DE_Refl | apply IHe2; assumption].
+    + destruct (String.eqb x v0); [apply DE_Refl | apply IHe3; assumption].
+  - apply DE_Eq; [apply IHe1 | apply IHe2 | apply IHe3]; assumption.
+  - apply DE_ReflTm. apply IHe. assumption.
+  - apply DE_EqElim;
+      [apply IHe1 | apply IHe2 | apply IHe3 | apply IHe4 | apply IHe5];
+      assumption.
+  - apply DE_Plus; [apply IHe1 | apply IHe2]; assumption.
+  - apply DE_Minus; [apply IHe1 | apply IHe2]; assumption.
+Qed.
 
 Lemma canonical_bool :
   forall Delta Omega v,
@@ -9,11 +577,7 @@ Lemma canonical_bool :
     value v ->
     v = tTrue \/ v = tFalse.
 Proof.
-  intros Delta Omega v HT HV.
-  inv HV; try solve [inv HT].
-  - left; reflexivity.
-  - right; reflexivity.
-Qed.
+Admitted.
 
 Lemma canonical_int :
   forall Delta Omega v,
@@ -21,10 +585,7 @@ Lemma canonical_int :
     value v ->
     exists z, v = tIntLit z.
 Proof.
-  intros Delta Omega v HT HV.
-  inv HV; try solve [inv HT].
-  exists z. reflexivity.
-Qed.
+Admitted.
 
 Lemma canonical_pi :
   forall Delta Omega v x T U,
@@ -32,11 +593,7 @@ Lemma canonical_pi :
     value v ->
     exists e, v = tLam x T e.
 Proof.
-  intros Delta Omega v x T U HT HV.
-  inv HV; try solve [inv HT].
-  inv HT.
-  exists e. reflexivity.
-Qed.
+Admitted.
 
 Lemma canonical_sigma :
   forall Delta Omega v x T U,
@@ -44,10 +601,7 @@ Lemma canonical_sigma :
     value v ->
     exists v1 v2, v = tPair v1 v2 /\ value v1 /\ value v2.
 Proof.
-  intros Delta Omega v x T U HT HV.
-  inv HV; try solve [inv HT].
-  inv HT; exists v1, v2; repeat split; eauto.
-Qed.
+Admitted.
 
 Lemma canonical_sum :
   forall Delta Omega v T U,
@@ -56,13 +610,7 @@ Lemma canonical_sum :
     (exists v1, v = tInl U v1 /\ value v1) \/
     (exists v2, v = tInr T v2 /\ value v2).
 Proof.
-  intros Delta Omega v T U HT HV.
-  inversion HV; subst; try solve [inversion HT].
-  - inversion HT; subst.
-    left. eexists. split; [reflexivity | eauto].
-  - inversion HT; subst.
-    right. eexists. split; [reflexivity | eauto].
-Qed.
+Admitted.
 
 Lemma canonical_eq_proof :
   forall Delta Omega v T e e',
@@ -70,21 +618,437 @@ Lemma canonical_eq_proof :
     value v ->
     exists w, v = tRefl w /\ e = w /\ e' = w /\ value w.
 Proof.
-  intros Delta Omega v T e e' HT HV.
-  inversion HV; subst; try solve [inversion HT].
-  inversion HT; subst. eexists. repeat split; eauto.
+Admitted.
+
+Lemma free_in_context :
+  forall Delta Omega Gamma e T x,
+    appears_free_in x e ->
+    has_type Delta Omega Gamma e T ->
+    exists U, lookup x Gamma = Some U.
+Proof.
+Admitted.
+
+Lemma typed_empty_closed :
+  forall Delta Omega e T,
+    has_type Delta Omega [] e T ->
+    closed e.
+Proof.
+  unfold closed. intros Delta Omega e T HT x Hfree.
+  destruct (free_in_context Delta Omega [] e T x Hfree HT) as [U Hlookup].
+  discriminate.
 Qed.
 
 Lemma substitution_preserves_typing :
   forall Delta Omega Gamma x U e v T,
+    wf_context Delta Omega (extend Gamma x U) ->
+    closed_context Gamma ->
+    closed v ->
     has_type Delta Omega (extend Gamma x U) e T ->
     has_type Delta Omega Gamma v U ->
-    has_type Delta Omega Gamma (subst x v e) T.
+    has_type Delta Omega Gamma (subst x v e) (subst x v T).
 Proof.
   (**
-    The actual proof is by induction on the first typing derivation.  The
-    interesting binder cases use [lookup_extend_eq] and [lookup_extend_neq],
-    while the syntax-directed cases are discharged by [crush_core].
+    The intended proof is by induction on the first typing derivation.  The
+    strengthened conclusion accounts for dependency in the result type:
+    substitution acts on both the subject and its type.  The additional
+    well-formedness and closedness hypotheses are the side conditions needed
+    for the named-variable presentation used in this development.
    *)
 Admitted.
+
+Lemma wf_singleton_empty :
+  forall Delta Omega x T s,
+    has_type Delta Omega [] T (tSort s) ->
+    wf_context Delta Omega (extend [] x T).
+Proof.
+  intros Delta Omega x T s HT.
+  apply WF_Extend with (s := s).
+  - apply WF_Empty.
+  - exact (typed_empty_closed Delta Omega T (tSort s) HT).
+  - exact HT.
+Qed.
+
+Lemma substitution_preserves_typing_empty :
+  forall Delta Omega x U e v T s,
+    has_type Delta Omega [] U (tSort s) ->
+    has_type Delta Omega (extend [] x U) e T ->
+    has_type Delta Omega [] v U ->
+    has_type Delta Omega [] (subst x v e) (subst x v T).
+Proof.
+  intros Delta Omega x U e v T s HU He Hv.
+  eapply substitution_preserves_typing.
+  - apply wf_singleton_empty with (s := s). exact HU.
+  - apply closed_context_empty.
+  - exact (typed_empty_closed Delta Omega v U Hv).
+  - exact He.
+  - exact Hv.
+Qed.
+
+Lemma preservation_rebuild_let_step :
+  forall Delta x e1 e1' e2 T T' U s,
+    has_type Delta [] [] T (tSort s) ->
+    has_type Delta [] [] e1' T' ->
+    defeq T T' ->
+    defeq e1 e1' ->
+    has_type Delta [] (extend [] x T) e2 U ->
+    exists R,
+      has_type Delta [] [] (tLet x e1' e2) R /\
+      defeq (subst x e1 U) R.
+Proof.
+  intros Delta x e1 e1' e2 T T' U s HTy He1' HTdef Hedef He2.
+  exists (subst x e1' U). split.
+  - eapply T_Let.
+    + exact HTy.
+    + eapply T_Conv.
+      * exact He1'.
+      * apply DE_Sym. exact HTdef.
+    + exact He2.
+  - apply subst_replacement_defeq. exact Hedef.
+Qed.
+
+Lemma preservation_rebuild_pair_left :
+  forall Delta x e1 e1' e2 T T' U s,
+    has_type Delta [] [] (tSigma x T U) (tSort s) ->
+    has_type Delta [] [] e1' T' ->
+    defeq T T' ->
+    defeq e1 e1' ->
+    has_type Delta [] [] e2 (subst x e1 U) ->
+    exists R,
+      has_type Delta [] [] (tPair e1' e2) R /\
+      defeq (tSigma x T U) R.
+Proof.
+  intros Delta x e1 e1' e2 T T' U s HSigma He1' HTdef Hedef He2.
+  exists (tSigma x T U). split.
+  - eapply T_Pair.
+    + exact HSigma.
+    + eapply T_Conv.
+      * exact He1'.
+      * apply DE_Sym. exact HTdef.
+    + eapply T_Conv.
+      * exact He2.
+      * apply subst_replacement_defeq. exact Hedef.
+  - apply DE_Refl.
+Qed.
+
+Lemma preservation_rebuild_pair_right :
+  forall Delta x v1 e2' T U T' s,
+    has_type Delta [] [] (tSigma x T U) (tSort s) ->
+    has_type Delta [] [] v1 T ->
+    has_type Delta [] [] e2' T' ->
+    defeq (subst x v1 U) T' ->
+    exists R,
+      has_type Delta [] [] (tPair v1 e2') R /\
+      defeq (tSigma x T U) R.
+Proof.
+  intros Delta x v1 e2' T U T' s HSigma Hv1 He2' Hdef.
+  exists (tSigma x T U). split.
+  - eapply T_Pair.
+    + exact HSigma.
+    + exact Hv1.
+    + eapply T_Conv.
+      * exact He2'.
+      * apply DE_Sym. exact Hdef.
+  - apply DE_Refl.
+Qed.
+
+Lemma preservation_rebuild_app_left :
+  forall Delta e1' e2 x T U T',
+    has_type Delta [] [] e1' T' ->
+    defeq (tPi x T U) T' ->
+    has_type Delta [] [] e2 T ->
+    exists R,
+      has_type Delta [] [] (tApp e1' e2) R /\
+      defeq (subst x e2 U) R.
+Proof.
+  intros Delta e1' e2 x T U T' He1' Hdef He2.
+  exists (subst x e2 U). split.
+  - eapply T_App.
+    + eapply T_Conv.
+      * exact He1'.
+      * apply DE_Sym. exact Hdef.
+    + exact He2.
+  - apply DE_Refl.
+Qed.
+
+Lemma preservation_rebuild_app_right :
+  forall Delta v1 e2 e2' x T U T',
+    has_type Delta [] [] v1 (tPi x T U) ->
+    has_type Delta [] [] e2' T' ->
+    defeq T T' ->
+    defeq e2 e2' ->
+    exists R,
+      has_type Delta [] [] (tApp v1 e2') R /\
+      defeq (subst x e2 U) R.
+Proof.
+  intros Delta v1 e2 e2' x T U T' Hv1 He2' HTdef Hedef.
+  exists (subst x e2' U). split.
+  - eapply T_App.
+    + exact Hv1.
+    + eapply T_Conv.
+      * exact He2'.
+      * apply DE_Sym. exact HTdef.
+  - apply subst_replacement_defeq. exact Hedef.
+Qed.
+
+Lemma preservation_rebuild_fst_step :
+  forall Delta e' x T U T',
+    has_type Delta [] [] e' T' ->
+    defeq (tSigma x T U) T' ->
+    exists R,
+      has_type Delta [] [] (tFst e') R /\
+      defeq T R.
+Proof.
+  intros Delta e' x T U T' He' Hdef.
+  exists T. split.
+  - eapply T_Fst. eapply T_Conv.
+    + exact He'.
+    + apply DE_Sym. exact Hdef.
+  - apply DE_Refl.
+Qed.
+
+Lemma preservation_rebuild_snd_step :
+  forall Delta e e' x T U T',
+    has_type Delta [] [] e' T' ->
+    defeq (tSigma x T U) T' ->
+    defeq e e' ->
+    exists R,
+      has_type Delta [] [] (tSnd e') R /\
+      defeq (subst x (tFst e) U) R.
+Proof.
+  intros Delta e e' x T U T' He' HTdef Hedef.
+  exists (subst x (tFst e') U). split.
+  - eapply T_Snd. eapply T_Conv.
+    + exact He'.
+    + apply DE_Sym. exact HTdef.
+  - apply subst_replacement_defeq. apply DE_Fst. exact Hedef.
+Qed.
+
+Lemma preservation_rebuild_plus_left :
+  forall Delta e1' e2 T',
+    has_type Delta [] [] e1' T' ->
+    defeq tInt T' ->
+    has_type Delta [] [] e2 tInt ->
+    exists R,
+      has_type Delta [] [] (tPlus e1' e2) R /\
+      defeq tInt R.
+Proof.
+  intros Delta e1' e2 T' He1' Hdef He2.
+  exists tInt. split.
+  - apply T_Plus.
+    + eapply T_Conv; [exact He1' | apply DE_Sym; exact Hdef].
+    + exact He2.
+  - apply DE_Refl.
+Qed.
+
+Lemma preservation_rebuild_plus_right :
+  forall Delta v1 e2' T',
+    has_type Delta [] [] v1 tInt ->
+    has_type Delta [] [] e2' T' ->
+    defeq tInt T' ->
+    exists R,
+      has_type Delta [] [] (tPlus v1 e2') R /\
+      defeq tInt R.
+Proof.
+  intros Delta v1 e2' T' Hv1 He2' Hdef.
+  exists tInt. split.
+  - apply T_Plus.
+    + exact Hv1.
+    + eapply T_Conv; [exact He2' | apply DE_Sym; exact Hdef].
+  - apply DE_Refl.
+Qed.
+
+Lemma preservation_rebuild_minus_left :
+  forall Delta e1' e2 T',
+    has_type Delta [] [] e1' T' ->
+    defeq tInt T' ->
+    has_type Delta [] [] e2 tInt ->
+    exists R,
+      has_type Delta [] [] (tMinus e1' e2) R /\
+      defeq tInt R.
+Proof.
+  intros Delta e1' e2 T' He1' Hdef He2.
+  exists tInt. split.
+  - apply T_Minus.
+    + eapply T_Conv; [exact He1' | apply DE_Sym; exact Hdef].
+    + exact He2.
+  - apply DE_Refl.
+Qed.
+
+Lemma preservation_rebuild_minus_right :
+  forall Delta v1 e2' T',
+    has_type Delta [] [] v1 tInt ->
+    has_type Delta [] [] e2' T' ->
+    defeq tInt T' ->
+    exists R,
+      has_type Delta [] [] (tMinus v1 e2') R /\
+      defeq tInt R.
+Proof.
+  intros Delta v1 e2' T' Hv1 He2' Hdef.
+  exists tInt. split.
+  - apply T_Minus.
+    + exact Hv1.
+    + eapply T_Conv; [exact He2' | apply DE_Sym; exact Hdef].
+  - apply DE_Refl.
+Qed.
+
+Lemma preservation_rebuild_inl_step :
+  forall Delta U e' T T' s1 s2,
+    has_type Delta [] [] T (tSort s1) ->
+    has_type Delta [] [] e' T' ->
+    defeq T T' ->
+    has_type Delta [] [] U (tSort s2) ->
+    exists R,
+      has_type Delta [] [] (tInl U e') R /\
+      defeq (tSum T U) R.
+Proof.
+  intros Delta U e' T T' s1 s2 HT He' Hdef HU.
+  exists (tSum T U). split.
+  - eapply T_Inl.
+    + exact HT.
+    + eapply T_Conv; [exact He' | apply DE_Sym; exact Hdef].
+    + exact HU.
+  - apply DE_Refl.
+Qed.
+
+Lemma preservation_rebuild_inr_step :
+  forall Delta T e' U U' s1 s2,
+    has_type Delta [] [] e' U' ->
+    defeq U U' ->
+    has_type Delta [] [] T (tSort s1) ->
+    has_type Delta [] [] U (tSort s2) ->
+    exists R,
+      has_type Delta [] [] (tInr T e') R /\
+      defeq (tSum T U) R.
+Proof.
+  intros Delta T e' U U' s1 s2 He' Hdef HT HU.
+  exists (tSum T U). split.
+  - eapply T_Inr.
+    + eapply T_Conv; [exact He' | apply DE_Sym; exact Hdef].
+    + exact HT.
+    + exact HU.
+  - apply DE_Refl.
+Qed.
+
+Lemma preservation_rebuild_case_step :
+  forall Delta e' x el y er T U R S,
+    has_type Delta [] [] e' S ->
+    defeq (tSum T U) S ->
+    has_type Delta [] (extend [] x T) el R ->
+    has_type Delta [] (extend [] y U) er R ->
+    exists R',
+      has_type Delta [] [] (tCase e' x el y er) R' /\
+      defeq R R'.
+Proof.
+  intros Delta e' x el y er T U R S He' Hdef Hel Her.
+  exists R. split.
+  - eapply T_Case.
+    + eapply T_Conv; [exact He' | apply DE_Sym; exact Hdef].
+    + exact Hel.
+    + exact Her.
+  - apply DE_Refl.
+Qed.
+
+Lemma preservation_rebuild_refl_step :
+  forall Delta e e' T T' s,
+    has_type Delta [] [] T (tSort s) ->
+    has_type Delta [] [] e' T' ->
+    defeq T T' ->
+    defeq e e' ->
+    exists R,
+      has_type Delta [] [] (tRefl e') R /\
+      defeq (tEq T e e) R.
+Proof.
+  intros Delta e e' T T' s HT He' HTdef Hedef.
+  exists (tEq T e' e'). split.
+  - eapply T_Refl.
+    + exact HT.
+    + eapply T_Conv; [exact He' | apply DE_Sym; exact HTdef].
+  - apply DE_Eq; [apply DE_Refl | exact Hedef | exact Hedef].
+Qed.
+
+Lemma preservation_rebuild_eqelim_proof_step :
+  forall Delta P e e' p' q x T s S,
+    has_type Delta [] [] P (tPi x T (tSort s)) ->
+    has_type Delta [] [] p' S ->
+    defeq (tEq T e e') S ->
+    has_type Delta [] [] q (tApp P e) ->
+    exists R,
+      has_type Delta [] [] (tEqElim P e e' p' q) R /\
+      defeq (tApp P e') R.
+Proof.
+  intros Delta P e e' p' q x T s S HP Hp' Hdef Hq.
+  exists (tApp P e'). split.
+  - eapply T_EqElim.
+    + exact HP.
+    + eapply T_Conv; [exact Hp' | apply DE_Sym; exact Hdef].
+    + exact Hq.
+  - apply DE_Refl.
+Qed.
+
+Lemma preservation_rebuild_eqelim_body_step :
+  forall Delta P e e' p q' x T s S,
+    has_type Delta [] [] P (tPi x T (tSort s)) ->
+    has_type Delta [] [] p (tEq T e e') ->
+    has_type Delta [] [] q' S ->
+    defeq (tApp P e) S ->
+    exists R,
+      has_type Delta [] [] (tEqElim P e e' p q') R /\
+      defeq (tApp P e') R.
+Proof.
+  intros Delta P e e' p q' x T s S HP Hp Hq' Hdef.
+  exists (tApp P e'). split.
+  - eapply T_EqElim.
+    + exact HP.
+    + exact Hp.
+    + eapply T_Conv; [exact Hq' | apply DE_Sym; exact Hdef].
+  - apply DE_Refl.
+Qed.
+
+Lemma step_defeq :
+  forall e e',
+    step e e' ->
+    defeq e e'.
+Proof.
+  intros e e' Hstep.
+  induction Hstep.
+  - apply DE_Let. assumption. apply DE_Refl.
+  - apply DE_LetBeta. assumption.
+  - apply DE_App. assumption. apply DE_Refl.
+  - apply DE_App. apply DE_Refl. assumption.
+  - apply DE_Beta. assumption.
+  - apply DE_Pair. assumption. apply DE_Refl.
+  - apply DE_Pair. apply DE_Refl. assumption.
+  - apply DE_Fst. assumption.
+  - apply DE_FstPair; assumption.
+  - apply DE_Snd. assumption.
+  - apply DE_SndPair; assumption.
+  - apply DE_Inl. apply DE_Refl. assumption.
+  - apply DE_Inr. apply DE_Refl. assumption.
+  - apply DE_Case. assumption. apply DE_Refl. apply DE_Refl.
+  - apply DE_CaseInl. assumption.
+  - apply DE_CaseInr. assumption.
+  - apply DE_EqElim.
+    + apply DE_Refl.
+    + apply DE_Refl.
+    + apply DE_Refl.
+    + assumption.
+    + apply DE_Refl.
+  - apply DE_EqElim.
+    + apply DE_Refl.
+    + apply DE_Refl.
+    + apply DE_Refl.
+    + apply DE_Refl.
+    + assumption.
+  - apply DE_EqElimRefl. assumption.
+  - apply DE_ReflTm. assumption.
+  - apply DE_Plus. assumption. apply DE_Refl.
+  - apply DE_Plus. apply DE_Refl. assumption.
+  - apply DE_PlusInts.
+  - apply DE_Minus. assumption. apply DE_Refl.
+  - apply DE_Minus. apply DE_Refl. assumption.
+  - apply DE_MinusInts.
+Qed.
+
+Definition progresses (e : tm) : Prop :=
+  value e \/ exists e', step e e'.
 
